\documentclass{article}
\usepackage{amsmath} % Để sử dụng môi trường toán học và lệnh aligned
\usepackage[vietnamese]{babel}

\begin{document}

\section{Bài 1}

\subsection{}

\subsubsection{$A= 1+3+5+7+\cdots+999$}

\[
\begin{aligned}
A &= \frac{(\frac{999-1}{2}+1)(999+1)}{2} \\
&= 250000
\end{aligned}
\]

\subsubsection{$A=2+4+6+8+\cdots+1024$}

\[
\begin{aligned}
A &= \frac{(\frac{1024-2}{2}+1)(1024+2)}{2} \\
&= 262656
\end{aligned}
\]

\subsubsection{$A=\sum_{i=3}^{n+1}1$}

\[
\begin{aligned}
A &= \underbrace{1+1+1+\cdots+1}_{\text{$n-1$ phần tử 1}} \\
&= \frac{(n+1)(n+2)}{2}-3 
\end{aligned}
\]


\subsubsection{$A=\sum_{i=3}^{n+1}i$}

\[
\begin{aligned}
A &= 3+4+5+\cdots+n+(n+1) \\
&= 1+2+3+\cdots+(n+1)-3 \\
&= \frac{(n+1)(n+2)}{2}-3 
\end{aligned}
\]

\subsubsection{$A=\sum_{i=0}^{n-1}i(i+1)$}

\[
\begin{aligned}
A &= \sum_{i=0}^{n-1}i^2+\sum_{i=0}^{n-1}i \\
&= \sum_{i=1}^{n-1}i^2+\sum_{i=1}^{n-1}i \\
&= \frac{(n-1)n(2n-1)}{6}+\frac{n(n-1)}{2} \\
&= \frac{(n-1)n(2n-1)}{6} + \frac{3n(n-1)}{6} \\
&= \frac{(n-1)n(2n-1 + 3)}{6} \\
&= \frac{(n-1)n(2n+2)}{6}
\end{aligned}
\]

\subsubsection{$A=\sum_{j=1}^{n}3^{j+1}$}

\[
\begin{aligned}
A &= 3^2 + 3^3 + \cdots + 3^n + 3^{n+1} \\
3A &= 3^3 + 3^4 + \cdots + 3^{n+1} + 3^{n+2} \\
\Rightarrow{} 2A &= 3A - 2A = 3^{n+2}-3^2 \\
\Rightarrow{} A &= \frac{3^{n+2}-3^2}{2} = \frac{(3^n-1)3^2}{2} \\
\end{aligned}
\]

\subsubsection{$A=\sum_{i=1}^{n}\sum_{j=1}^{n}ij$}

\[
\begin{aligned}
A &= \sum_{i=1}^{n}i(\sum_{j=1}^{n}j) \\
&= \frac{n(n+1)}{2}\sum_{i=1}^{n}i \\
&= \frac{n(n+1)}{2}\cdot\frac{n(n+1)}{2} \\
&= \frac{n^2{(n+1)}^2}{4}
\end{aligned}
\]

\subsubsection{$A=\sum_{i=1}^{n}\frac{1}{i(i+1)}$}

\[
\begin{aligned}
A &= \sum_{i=1}^{n}(\frac{1}{i}-\frac{1}{i+1}) \\
&= (1-\frac{1}{2})+(\frac{1}{2}-\frac{1}{3})+(\frac{1}{3}-\frac{1}{4})+(\frac{1}{4}-\frac{1}{5})+\cdots+(\frac{1}{n}-\frac{1}{n+1}) \\
&= 1-\frac{1}{n+1} \\
&= \frac{n}{n+1}
\end{aligned}
\]

\subsubsection{$A=\sum_{j \in \{2, 3, 5\}} (j^2 + j)$}

\[
\begin{aligned}
A &= (2^2+2)+(3^2+3)+(5^2+5) \\
&= 48
\end{aligned}
\]

\subsubsection{$A=\sum_{i=1}^{m}\sum_{j=0}^{n}\sum_{k=0}^{100}(i+j)$}

\[
\begin{aligned}
A &= \sum_{i=1}^{m}\sum_{j=0}^{n}(\sum_{k=0}^{100}(i+j)) \\
&= \sum_{i=1}^{m}\sum_{j=0}^{n}((i+j)\sum_{k=0}^{100}1) \\
&= 101\sum_{i=1}^{m}\sum_{j=0}^{n}(i+j) \\
&= 101\sum_{i=1}^{m}(i\sum_{j=0}^{n}1+\sum_{j=0}^{n}j) \\
&= 101\sum_{i=1}^{m}((n+1)i+\frac{n(n+1)}{2}) \\
&= 101(\sum_{i=1}^{m}(n+1)i+\sum_{i=1}^{m}\frac{n(n+1)}{2}) \\
&= 101(\frac{(n+1)m(m+1)}{2}+\frac{n(n+1)m}{2}) \\
&= \frac{101}{2}(n+1)m(m+1+n)
\end{aligned}
\]

\subsection{}

\subsubsection{$A=\sum_{i=0}^{n-1}{(i^2+1)}^2$}

\[
\begin{aligned}
A &= \sum_{i=0}^{n-1}(i^4+2i+1) \\
&= \sum_{i=0}^{n-1}i^4+\sum_{i=0}^{n-1}2i+\sum_{i=0}^{n-1}1 \\
&\approx \frac{1}{5}{(n-1)}^5+\frac{(n-1)n(2n-1)}{3}+n
\end{aligned}
\]

\subsubsection{$A=\sum_{i=2}^{n-1}\lg i^2$}

\[
\begin{aligned}
A &= \sum_{i=2}^{n-1}\lg 2i \\
&= 2\sum_{i=2}^{n-1}\lg i \\
&\approx (n-1)\lg(n-1)
\end{aligned}
\]

\subsubsection{$A=\sum_{i=1}^{n}(i+1)2^{i-1}$}

\[
\begin{aligned}
A &= \frac{1}{2}\sum_{i=1}^{n}(i+1)2^i \\
&= \frac{1}{2}\sum_{i=1}^{n}i2^i + \frac{1}{2}\sum_{i=1}^{n}2^i \\
&= \frac{1}{2}[(n-1)2^{n+1}+2] +\frac{1}{2}(2^{n+1}-2) \\
&= (n-1)2^n+2^n \\
&= n2^n
\end{aligned}    
\]

\subsubsection{$A=\sum_{i=0}^{n-1}\sum_{j=0}^{i-1}(i+j)$}

\[
\begin{aligned}
A &= \sum_{i=0}^{n-1}(\sum_{j=0}^{i-1}i+\sum_{j=0}^{i-1}j) \\
&= \sum_{i=0}^{n-1}(i^2+\frac{(i-1)i}{2}) \\
&= \sum_{i=0}^{n-1}(\frac{3}{2}i^2-\frac{1}{2}i) \\
&= \sum_{i=0}^{n-1}\frac{3}{2}i^2 - \sum_{i=0}^{n-1}\frac{1}{2}i \\
&= \frac{(n-1)n(2n-1)}{4}-\frac{(n-1)n}{4} \\
&= \frac{n{(n-1)}^2}{2} 
\end{aligned}
\]

\section{Bài 2}
- Phép gán: {$2+2n+$}
\end{document}